src/ManCompSoundness.v
@@ -22,9 +22,7 @@ Definition lib_supports_manifest (al : AM_Library) (am : Manifest) : Prop :=
   (forall (up : Plc), In_set up am.(uuidPlcs) -> 
     exists b, Maps.map_get al.(Lib_Plcs) up = Some b) /\
   (forall (pkp : Plc), In_set pkp am.(pubKeyPlcs) -> 
-    exists b, Maps.map_get al.(Lib_PubKeys) pkp = Some b) /\
-  (forall (a : ASP_ID), In_set a am.(appraisal_asps) -> 
-    exists aloc, Maps.map_get al.(Lib_ASPs) a = Some aloc).
+    exists b, Maps.map_get al.(Lib_PubKeys) pkp = Some b).
 
 Ltac unfolds :=
   (* repeat monad_unfold; *)
@@ -506,13 +504,7 @@ Definition manifest_support_am_config (m : Manifest) (ac : AM_Config) : Prop :=
     (exists errStr, ac.(plcCb) p = errC (Runtime errStr))) /\
   (forall p, In_set p (m.(pubKeyPlcs)) ->
     (exists res, ac.(pubKeyCb) p = resultC res) \/
-    (exists errStr, ac.(pubKeyCb) p = errC (Runtime errStr))) /\
-
-    (forall a, In_set a (m.(appraisal_asps)) -> 
-    forall l targ targid ev,
-    (exists res, ac.(aspCb) (asp_paramsC a l targ targid) ev = resultC res) \/
-    (exists errStr, ac.(aspCb) (asp_paramsC a l targ targid) ev = errC (Runtime errStr))).
-
+    (exists errStr, ac.(pubKeyCb) p = errC (Runtime errStr))).
 
 Theorem manifest_support_am_config_compiler : forall absMan amLib aspBin,
   lib_supports_manifest amLib absMan ->
@@ -949,7 +941,6 @@ Proof.
           {|
             my_abstract_plc := my_abstract_plc;
             asps := asps;
-            appraisal_asps := appraisal_asps;
             uuidPlcs := manset_add p uuidPlcs;
             pubKeyPlcs := pubKeyPlcs;
             targetPlcs := targetPlcs;
@@ -961,7 +952,6 @@ Proof.
           {|
             my_abstract_plc := my_abstract_plc;
             asps := asps;
-            appraisal_asps := appraisal_asps;
             uuidPlcs := manset_add p uuidPlcs;
             pubKeyPlcs := pubKeyPlcs;
             targetPlcs := targetPlcs;
@@ -981,7 +971,6 @@ Proof.
          {|
            my_abstract_plc := my_abstract_plc;
            asps := asps;
-           appraisal_asps := appraisal_asps;
            uuidPlcs := manset_add p uuidPlcs;
            pubKeyPlcs := pubKeyPlcs;
            targetPlcs := targetPlcs;
@@ -989,7 +978,6 @@ Proof.
          |}) p0 = Some {|
          my_abstract_plc := my_abstract_plc;
          asps := asps;
-         appraisal_asps := appraisal_asps;
          uuidPlcs := manset_add p uuidPlcs;
          pubKeyPlcs := pubKeyPlcs;
          targetPlcs := targetPlcs;
@@ -1004,7 +992,6 @@ Proof.
       specialize H with (m1 := {|
         my_abstract_plc := my_abstract_plc;
         asps := asps;
-        appraisal_asps := appraisal_asps;
         uuidPlcs := @manset_add _ Eq_Class_ID_Type p uuidPlcs;
         pubKeyPlcs := pubKeyPlcs;
         targetPlcs := targetPlcs;
@@ -1019,30 +1006,28 @@ Proof.
 
       +
 
-      subst.
+      subst; simpl in *.
 
       assert (Environment_subset 
-      (map_set e p0
+      (map_set e my_abstract_plc
           {|
             my_abstract_plc := my_abstract_plc;
-            asps := asps;
-            appraisal_asps := appraisal_asps;
-            uuidPlcs := manset_add p uuidPlcs;
-            pubKeyPlcs := pubKeyPlcs;
-            targetPlcs := targetPlcs;
-            policy := policy
+            asps := manifest_set_empty;
+            uuidPlcs := [p];
+            pubKeyPlcs := manifest_set_empty;
+            targetPlcs := manifest_set_empty;
+            policy := empty_PolicyT;
           |})
 
           (manifest_generator' p t
-       (map_set e p0
+      (map_set e my_abstract_plc
           {|
             my_abstract_plc := my_abstract_plc;
-            asps := asps;
-            appraisal_asps := appraisal_asps;
-            uuidPlcs := manset_add p uuidPlcs;
-            pubKeyPlcs := pubKeyPlcs;
-            targetPlcs := targetPlcs;
-            policy := policy
+            asps := manifest_set_empty;
+            uuidPlcs := [p];
+            pubKeyPlcs := manifest_set_empty;
+            targetPlcs := manifest_set_empty;
+            policy := empty_PolicyT;
           |}))
       
       ).
@@ -1051,47 +1036,37 @@ Proof.
       }
       unfold Environment_subset in *.
 
-
       assert (
         map_get
-      (map_set e p0
+      (map_set e my_abstract_plc
          {|
            my_abstract_plc := my_abstract_plc;
-           asps := asps;
-           appraisal_asps := appraisal_asps;
-           uuidPlcs := manset_add p uuidPlcs;
-           pubKeyPlcs := pubKeyPlcs;
-           targetPlcs := targetPlcs;
-           policy := policy
-         |}) p0 = Some {|
-         my_abstract_plc := my_abstract_plc;
-         asps := asps;
-         appraisal_asps := appraisal_asps;
-         uuidPlcs := manset_add p uuidPlcs;
-         pubKeyPlcs := pubKeyPlcs;
-         targetPlcs := targetPlcs;
-         policy := policy
+           asps := manifest_set_empty;
+           uuidPlcs := [p];
+           pubKeyPlcs := manifest_set_empty;
+           targetPlcs := manifest_set_empty;
+           policy := empty_PolicyT;
+         |}) my_abstract_plc = Some {|
+           my_abstract_plc := my_abstract_plc;
+           asps := manifest_set_empty;
+           uuidPlcs := [p];
+           pubKeyPlcs := manifest_set_empty;
+           targetPlcs := manifest_set_empty;
+           policy := empty_PolicyT;
        |}
       ).
       {
         eapply mapC_get_works.
-
       }
 
-      specialize H with (m1 := {|
-        my_abstract_plc := my_abstract_plc;
-        asps := asps;
-        appraisal_asps := appraisal_asps;
-        uuidPlcs := @manset_add _ Eq_Class_ID_Type p uuidPlcs;
-        pubKeyPlcs := pubKeyPlcs;
-        targetPlcs := targetPlcs;
-        policy := policy
-      |}) (p := p0).
+      pose proof (H _ _ H0).
+
       find_apply_hyp_hyp.
       destruct_conjs.
+      eexists.
+      erewrite H2.
 
-      exists H0.
-      eauto.
+      simpl in *; intuition.
 
     - (* lseq case *)
       ff.
@@ -1415,7 +1390,6 @@ Proof.
               {|
                 my_abstract_plc := my_abstract_plc;
                 asps := asps;
-                appraisal_asps := appraisal_asps;
                 uuidPlcs := manset_add p uuidPlcs;
                 pubKeyPlcs := pubKeyPlcs;
                 targetPlcs := targetPlcs;
@@ -1439,7 +1413,6 @@ Proof.
               {|
                 my_abstract_plc := p0;
                 asps := manifest_set_empty;
-                appraisal_asps := manifest_set_empty;
                 uuidPlcs := manset_add p manifest_set_empty;
                 pubKeyPlcs := manifest_set_empty;
                 targetPlcs := manifest_set_empty; (* v; *)
@@ -2214,12 +2187,14 @@ Lemma mangen_plcTerm_subset_end_to_end_mangen : forall ts t tp,
   In (t, tp) ts ->
   (forall m m' p,
     map_get (mangen_plcTerm_list_union ts) p = Some m' ->
-    forall ls, map_get (end_to_end_mangen' ls ts) p = Some m ->
-    manifest_subset m' m
+    forall ls al env, 
+      end_to_end_mangen' ls ts al = resultC env ->
+      map_get env p = Some m ->
+      manifest_subset m' m
   ).
 Proof.
-  intuition; unfold end_to_end_mangen' in *;
-  eapply manifest_env_union_always_subset in H1; intuition.
+  intuition; unfold end_to_end_mangen' in *; ff;
+  find_eapply_lem_hyp manifest_env_union_always_subset; intuition.
 Qed.
 Global Hint Resolve mangen_plcTerm_subset_end_to_end_mangen : core.
 
@@ -2227,35 +2202,19 @@ Lemma mangen_subset_end_to_end_mangen : forall ts t tp,
   In (t, tp) ts ->
   (forall m m' p,
     map_get (manifest_generator t tp) p = Some m' ->
-    forall ls, map_get (end_to_end_mangen' ls ts) p = Some m ->
-    manifest_subset m' m
+    forall ls al env, 
+      end_to_end_mangen' ls ts al = resultC env ->
+      map_get env p = Some m ->
+      manifest_subset m' m
   ).
 Proof.
   intuition.
   assert (exists m'', map_get (mangen_plcTerm_list_union ts) p = Some m''). eapply mangen_plcTerm_list_exists; eauto.
   break_exists.
-  pose proof (mangen_plcTerm_list_subsumes ts p x H2 t tp H _ H0).
-  pose proof (mangen_plcTerm_subset_end_to_end_mangen ts t tp H m x p H2 ls H1).
+  pose proof (mangen_plcTerm_list_subsumes ts p x H3 t tp H _ H0).
   eapply manifest_subset_trans; eauto.
 Qed.
 Global Hint Resolve mangen_subset_end_to_end_mangen : core.
-
-Lemma mangen_subsets_of_end_to_end_mangen : forall ts t tp,
-  In (t, tp) ts ->
-  (forall m m' p,
-    map_get (manifest_generator t tp) p = Some m' ->
-    forall ls, map_get (end_to_end_mangen' ls ts) p = Some m ->
-    manifest_subset m' m
-  ).
-Proof.
-  intuition.
-  assert (exists m'', map_get (mangen_plcTerm_list_union ts) p = Some m''). eapply mangen_plcTerm_list_exists; eauto.
-  break_exists.
-  pose proof (mangen_plcTerm_list_subsumes ts p x H2 t tp H _ H0).
-  pose proof (mangen_plcTerm_subset_end_to_end_mangen ts t tp H m x p H2 ls H1).
-  eapply manifest_subset_trans; eauto.
-Qed.
-Global Hint Resolve mangen_subsets_of_end_to_end_mangen : core.
 
 Lemma always_a_man_gen_exists : forall t p tp,
   In p (places tp t) ->
@@ -2268,7 +2227,9 @@ Qed.
 Global Hint Resolve always_a_man_gen_exists : core.
 
 Lemma mangen_exists_end_to_end_mangen : forall ts ls p m,
-  map_get (end_to_end_mangen' ls ts) p = Some m ->
+  forall al env,
+    end_to_end_mangen' ls ts al = resultC env ->
+    map_get env p = Some m ->
   (forall t tp,
     In (t, tp) ts ->
     In p (places tp t) ->
@@ -2396,7 +2357,9 @@ Qed.
 Global Hint Resolve supports_am_mancomp_subset : core.
 
 Lemma end_to_end_mangen_supports_all : forall ts ls p m,
-  map_get (end_to_end_mangen' ls ts) p = Some m ->
+  forall al env,
+    end_to_end_mangen' ls ts al = resultC env ->
+    map_get env p = Some m ->
   (forall t tp, 
     In (t, tp) ts ->
     In p (places tp t) ->
@@ -2407,17 +2370,19 @@ Lemma end_to_end_mangen_supports_all : forall ts ls p m,
   ).
 Proof.
   intuition.
-  pose proof (mangen_exists_end_to_end_mangen _ _ _ _ H _ _ H0 H1 _ H2).
+  pose proof (mangen_exists_end_to_end_mangen _ _ _ _ _ _ H H0 _ _ H1 H2 _ H3).
   break_exists.
-  pose proof (mangen_subset_end_to_end_mangen _ _ _ H0 _ _ _ H3 _ H).
+  pose proof (mangen_subset_end_to_end_mangen _ _ _ H1 _ _ _ H4 _ _ _ H H0).
   pose proof manifest_supports_term_sub.
-  eapply (man_gen_old_always_supports) in H3 as H'; eauto.
+  pose proof (man_gen_old_always_supports _ _ _ _ _ _ H4 H2 H3).
+  eauto.
 Qed.
 Global Hint Resolve end_to_end_mangen_supports_all : core.
 
 Theorem manifest_generator_compiler_soundness_distributed_multiterm' : forall t ts ls tp p absMan amLib amConf aspBin,
-  (* map_get (manifest_generator t tp) p = Some absMan -> *)
-  map_get (end_to_end_mangen' ls ts) p = Some absMan -> 
+forall env,
+  end_to_end_mangen' ls ts amLib = resultC env ->
+  map_get env p = Some absMan ->
   In (t,tp) ts ->
   (* In p (places tp t) -> *)
   lib_supports_manifest amLib absMan ->
@@ -2453,7 +2418,7 @@ Proof.
     * (* NOTE: This is the important one, substitute proof of any manifest here *)
       assert (In p (places tp t)). {
         eapply in_plc_term; intuition; subst.
-        rewrite H5 in H4; simpl in *; intuition.
+        find_rewrite; eauto.
       }
       eapply end_to_end_mangen_supports_all; eauto.
   - match goal with
@@ -2568,9 +2533,9 @@ Proof.
 Qed.
 
 
-Theorem manifest_generator_compiler_soundness_distributed_multiterm : forall t ts ls tp p absMan amLib amConf aspBin,
-  (* map_get (manifest_generator t tp) p = Some absMan -> *)
-  map_get (end_to_end_mangen ls ts) p = Some absMan -> 
+Theorem manifest_generator_compiler_soundness_distributed_multiterm : forall t ts ls tp p absMan amLib amConf aspBin env,
+  end_to_end_mangen ls ts amLib = resultC env ->
+  map_get env p = Some absMan -> 
   In (t,tp) ts ->
   (* In p (places tp t) -> *)
   lib_supports_manifest amLib absMan ->
@@ -2596,12 +2561,13 @@ Theorem manifest_generator_compiler_soundness_distributed_multiterm : forall t t
     ).
 Proof.
   intros.
-  unfold end_to_end_mangen in H.
-  eapply exists_manifest_subset_update_pubkeys_env in H.
+  unfold end_to_end_mangen in H; ff; simpl in *.
+  pose proof (exists_manifest_subset_update_pubkeys_env _ _ _ _ H0).
   destruct_conjs.
-  eapply exists_manifest_subset_update_knowsOf_myPlc_env in H5.
+  find_eapply_lem_hyp exists_manifest_subset_update_knowsOf_myPlc_env.
   destruct_conjs.
   eapply manifest_generator_compiler_soundness_distributed_multiterm'.
+  eassumption.
   eassumption.
   eassumption.
   eapply lib_supports_manifest_subset.
@@ -2611,7 +2577,6 @@ Proof.
   eassumption.
   reflexivity.
   eapply supports_am_mancomp_subset.
-  rewrite H2.
   eassumption.
   eapply manifest_subset_trans.
   eassumption.
