src/Manifest.v
@@ -86,7 +86,6 @@ Definition empty_PolicyT : PolicyT := [].
     my_abstract_plc   : Plc ; 
 
     asps              : manifest_set ASP_ID; 
-    appraisal_asps    : manifest_set ASP_ID ;
     uuidPlcs          : manifest_set Plc ;
     pubKeyPlcs        : manifest_set Plc ;
     targetPlcs        : manifest_set Plc ;
@@ -97,7 +96,6 @@ Definition empty_PolicyT : PolicyT := [].
   Definition empty_Manifest : Manifest :=
     Build_Manifest 
       empty_Manifest_Plc 
-      manifest_set_empty
       manifest_set_empty
       manifest_set_empty
       manifest_set_empty
@@ -122,20 +120,8 @@ Record AM_Config : Type :=
   mkAmConfig {
     absMan : Manifest ;
     am_clone_addr : UUID ;
+    ASP_to_APPR_ASP_Map : MapC ASP_ID ASP_ID ;
     aspCb : (ASPCallback DispatcherErrors) ;
     plcCb : PlcCallback ;
     pubKeyCb : PubKeyCallback ;
   }.
-
-Definition empty_aspCb (ps:ASP_PARAMS) (rawev:RawEv) 
-    : ResultT RawEv DispatcherErrors := 
-  errC Unavailable.
-
-  Definition empty_am_config : AM_Config :=
-  mkAmConfig 
-    empty_Manifest
-    default_uuid
-    empty_aspCb
-    (fun x => errC Unavailable)
-    (fun x => errC Unavailable).
-
