src/Manifest_Union.v
@@ -10,41 +10,17 @@ Import ListNotations.
 
 Definition manifest_union (m1:Manifest) (m2:Manifest) : Manifest := 
     match (m1, m2) with 
-    | ((Build_Manifest myPlc asps1 app_asps1 uuidPlcs1 pubKeyPlcs1 targPlcs1 myPol),
-       (Build_Manifest _     asps2 app_asps2 uuidPlcs2 pubKeyPlcs2 targPlcs2 _    )) => 
+    | ((Build_Manifest myPlc asps1 uuidPlcs1 pubKeyPlcs1 targPlcs1 myPol),
+       (Build_Manifest _     asps2 uuidPlcs2 pubKeyPlcs2 targPlcs2 _    )) => 
 
        Build_Manifest
         myPlc 
         (manset_union asps1 asps2)
-        (manset_union app_asps1 app_asps2)
         (manset_union uuidPlcs1 uuidPlcs2)
         (manset_union pubKeyPlcs1 pubKeyPlcs2)
         (manset_union targPlcs1 targPlcs2)
         myPol
     end.
-
-(*
-Definition env_places (e:EnvironmentM) : list Plc.
-Admitted.
-*)
-
-(*
-
-Definition get_env_nofail (e:EnvironmentM) (p:Plc) : Manifest := 
-  match (map_get e p) with 
-  | Some m => m 
-  | _ => empty_Manifest
-  end.
-
-
-
-Definition union_single_plc_envs (e1:EnvironmentM) (e2:EnvironmentM) (p:Plc) : Manifest := 
-  manifest_union (get_env_nofail e1 p) (get_env_nofail e2 p).
-
-Definition environment_union' (e1:EnvironmentM) (e2:EnvironmentM) (p:Plc) (e':EnvironmentM) : EnvironmentM := 
-  let pman := (union_single_plc_envs e1 e2 p) in 
-    map_set e' p pman.
-*)
 
 Definition environment_union'' (p:Plc) (m1:Manifest) (e2:EnvironmentM) : EnvironmentM := 
   match (map_get e2 p) with 
@@ -53,7 +29,6 @@ Definition environment_union'' (p:Plc) (m1:Manifest) (e2:EnvironmentM) : Environ
       map_set e2 p new_man 
   | None => map_set e2 p m1
   end.
-
 
                                       (*  B  *)            (*  A  *)        (*  A  *)
 Definition env_union_helper (e1_pr:(Plc*Manifest)) (e2:EnvironmentM) : EnvironmentM := 
